rocq/div/sd.v
@@ -109,7 +109,7 @@ End IN.
 (* ----------------------------------------------------------- *)
 (** * Proof of equivalence for the type-and-effect systems *)
 
-Section Equivalence.
+Section IN_Equivalence.
 
 
 Fixpoint IN_to_Eff {n : nat} (Γ : Ctx n) e τ ε1 :
@@ -143,6 +143,106 @@ Proof.
   eapply IN.t_sub; eauto.
 Qed.
 
+End IN_Equivalence.
 
 
-End Equivalence.
+
+Module OUT.
+
+Definition lub (e1 : Eff) (e2 : Eff) := 
+  match e1 , e2 with 
+  | Top , _ => Top
+  | _ , Top => Top
+  | Bot, Bot => Bot
+  end.
+
+(* LUB calculates a least upper bound. *)
+Lemma lub_ub1 e1 e2 : e1 <: lub e1 e2.
+Proof. destruct e1; destruct e2; cbn; done. Qed.
+Lemma lub_ube e1 e2 : e2 <: lub e1 e2.
+Proof. destruct e1; destruct e2; cbn; done. Qed.
+Lemma lub_least e1 e2 e : e1 <: e -> e2 <: e -> lub e1 e2 <: e.
+Proof. destruct e1; destruct e2; destruct e; done. Qed.
+
+
+Inductive typing_val {n} (Γ : Ctx n) : Val n -> Ty 0 -> Prop := 
+  | t_var x : 
+    typing_val Γ (var x) (Γ x)
+
+  | t_zero : 
+    typing_val Γ zero Nat
+
+  | t_succ k : 
+    typing_val Γ k Nat ->
+    typing_val Γ (succ k) Nat
+
+  | t_pair v1 v2 τ1 τ2 ε : 
+    typing_val Γ v1 τ1 ->
+    typing_val Γ v2 τ2 -> 
+    typing_val Γ (prod v1 v2) (Prod ε τ1 τ2)
+
+  | t_inj1 v τ1 τ2 : 
+    typing_val Γ v τ1 ->
+    typing_val Γ (inj true v) (Sum τ1 τ2)
+
+  | t_inj2 v τ1 τ2 : 
+    typing_val Γ v τ2 ->
+    typing_val Γ (inj false v) (Sum τ1 τ2)
+
+
+  | t_rec v τ : 
+    allows_rec_ty τ = true ->
+    typing_val (τ .: Γ) v τ -> 
+    typing_val Γ (rec v) τ
+
+  | t_fold v τ : 
+    typing_val Γ v (τ [(Mu τ) ..]) ->
+    typing_val Γ (fold v) (Mu τ)
+
+
+with typing {n} (Γ : Ctx n) : Tm n -> Ty 0 -> Eff -> Prop := 
+  | t_ret v τ :
+    typing_val Γ v τ ->
+    typing Γ (ret v) τ ⊥
+
+  | t_let e1 e2 τ1 τ2 ε1 ε2 :
+    typing Γ e1 τ1 ε1 ->
+    typing (τ1 .: Γ) e2 τ2 ε2 ->
+    typing Γ (let_ e1 e2) τ2 (ε1 ⊕ ε2) 
+
+
+ | t_unfold v τ : 
+    typing_val Γ v (Mu τ) ->
+    typing Γ (unfold v) (τ [(Mu τ) ..]) ⊤
+.
+
+Definition t_var' {n} (Γ : Ctx n) x τ   : Γ x = τ -> typing_val Γ (var x) τ.
+intros <-. eapply t_var. Qed.
+
+#[export] Hint Resolve t_var' : rec.
+
+#[export] Hint Constructors typing_val typing : rec.
+
+  
+End OUT.
+
+Module OUT_Equivalence.
+
+Fixpoint OUT_to_Eff {n : nat} (Γ : Ctx n) e τ ε1 :
+  OUT.typing Γ e τ ε1 -> div.typing Γ e τ ε1
+with OUT_to_Eff_val {n : nat} (Γ : Ctx n) v τ :
+  OUT.typing_val Γ v τ -> div.typing_val Γ v τ.
+Proof. 
+(* FILL IN HERE *) Admitted.
+
+Fixpoint Eff_to_OUT {n : nat} (Γ : Ctx n) e τ ε1 :
+  div.typing Γ e τ ε1 -> exists ε, OUT.typing Γ e τ ε /\ ε <: ε1
+with Eff_to_OUT_val {n : nat} (Γ : Ctx n) v τ :
+  div.typing_val Γ v τ -> OUT.typing_val Γ v τ.
+Proof.
+(* FILL IN HERE *) Admitted.
+
+End OUT_Equivalence.
+
+
+
