rocq/rec/syntax.v
@@ -7,24 +7,33 @@ Module Core.
 
 Inductive Val (n_Val : nat) : Type :=
   | var : fin n_Val -> Val n_Val
+  | unit : Val n_Val
+  | abs : Tm (S n_Val) -> Val n_Val
   | zero : Val n_Val
   | succ : Val n_Val -> Val n_Val
   | prod : Val n_Val -> Val n_Val -> Val n_Val
   | inj : bool -> Val n_Val -> Val n_Val
-  | abs : Tm (S n_Val) -> Val n_Val
   | rec : Val (S n_Val) -> Val n_Val
   | fold : Val n_Val -> Val n_Val
 with Tm (n_Val : nat) : Type :=
   | ret : Val n_Val -> Tm n_Val
   | let_ : Tm n_Val -> Tm (S n_Val) -> Tm n_Val
+  | app : Val n_Val -> Val n_Val -> Tm n_Val
   | ifz : Val n_Val -> Tm n_Val -> Tm (S n_Val) -> Tm n_Val
   | prj : bool -> Val n_Val -> Tm n_Val
-  | split : Val n_Val -> Tm (S (S n_Val)) -> Tm n_Val
   | case : Val n_Val -> Tm (S n_Val) -> Tm (S n_Val) -> Tm n_Val
-  | app : Val n_Val -> Val n_Val -> Tm n_Val
-  | unfold : Val n_Val -> Tm n_Val
-  | box : Val n_Val -> Tm n_Val
-  | bind : Tm n_Val -> Tm (S n_Val) -> Tm n_Val.
+  | unfold : Val n_Val -> Tm n_Val.
+
+Lemma congr_unit {m_Val : nat} : unit m_Val = unit m_Val.
+Proof.
+exact (eq_refl).
+Qed.
+
+Lemma congr_abs {m_Val : nat} {s0 : Tm (S m_Val)} {t0 : Tm (S m_Val)}
+  (H0 : s0 = t0) : abs m_Val s0 = abs m_Val t0.
+Proof.
+exact (eq_trans eq_refl (ap (fun x => abs m_Val x) H0)).
+Qed.
 
 Lemma congr_zero {m_Val : nat} : zero m_Val = zero m_Val.
 Proof.
@@ -53,12 +62,6 @@ exact (eq_trans (eq_trans eq_refl (ap (fun x => inj m_Val x s1) H0))
          (ap (fun x => inj m_Val t0 x) H1)).
 Qed.
 
-Lemma congr_abs {m_Val : nat} {s0 : Tm (S m_Val)} {t0 : Tm (S m_Val)}
-  (H0 : s0 = t0) : abs m_Val s0 = abs m_Val t0.
-Proof.
-exact (eq_trans eq_refl (ap (fun x => abs m_Val x) H0)).
-Qed.
-
 Lemma congr_rec {m_Val : nat} {s0 : Val (S m_Val)} {t0 : Val (S m_Val)}
   (H0 : s0 = t0) : rec m_Val s0 = rec m_Val t0.
 Proof.
@@ -85,6 +88,14 @@ exact (eq_trans (eq_trans eq_refl (ap (fun x => let_ m_Val x s1) H0))
          (ap (fun x => let_ m_Val t0 x) H1)).
 Qed.
 
+Lemma congr_app {m_Val : nat} {s0 : Val m_Val} {s1 : Val m_Val}
+  {t0 : Val m_Val} {t1 : Val m_Val} (H0 : s0 = t0) (H1 : s1 = t1) :
+  app m_Val s0 s1 = app m_Val t0 t1.
+Proof.
+exact (eq_trans (eq_trans eq_refl (ap (fun x => app m_Val x s1) H0))
+         (ap (fun x => app m_Val t0 x) H1)).
+Qed.
+
 Lemma congr_ifz {m_Val : nat} {s0 : Val m_Val} {s1 : Tm m_Val}
   {s2 : Tm (S m_Val)} {t0 : Val m_Val} {t1 : Tm m_Val} {t2 : Tm (S m_Val)}
   (H0 : s0 = t0) (H1 : s1 = t1) (H2 : s2 = t2) :
@@ -104,14 +115,6 @@ exact (eq_trans (eq_trans eq_refl (ap (fun x => prj m_Val x s1) H0))
          (ap (fun x => prj m_Val t0 x) H1)).
 Qed.
 
-Lemma congr_split {m_Val : nat} {s0 : Val m_Val} {s1 : Tm (S (S m_Val))}
-  {t0 : Val m_Val} {t1 : Tm (S (S m_Val))} (H0 : s0 = t0) (H1 : s1 = t1) :
-  split m_Val s0 s1 = split m_Val t0 t1.
-Proof.
-exact (eq_trans (eq_trans eq_refl (ap (fun x => split m_Val x s1) H0))
-         (ap (fun x => split m_Val t0 x) H1)).
-Qed.
-
 Lemma congr_case {m_Val : nat} {s0 : Val m_Val} {s1 : Tm (S m_Val)}
   {s2 : Tm (S m_Val)} {t0 : Val m_Val} {t1 : Tm (S m_Val)}
   {t2 : Tm (S m_Val)} (H0 : s0 = t0) (H1 : s1 = t1) (H2 : s2 = t2) :
@@ -123,32 +126,10 @@ exact (eq_trans
          (ap (fun x => case m_Val t0 t1 x) H2)).
 Qed.
 
-Lemma congr_app {m_Val : nat} {s0 : Val m_Val} {s1 : Val m_Val}
-  {t0 : Val m_Val} {t1 : Val m_Val} (H0 : s0 = t0) (H1 : s1 = t1) :
-  app m_Val s0 s1 = app m_Val t0 t1.
-Proof.
-exact (eq_trans (eq_trans eq_refl (ap (fun x => app m_Val x s1) H0))
-         (ap (fun x => app m_Val t0 x) H1)).
-Qed.
-
 Lemma congr_unfold {m_Val : nat} {s0 : Val m_Val} {t0 : Val m_Val}
   (H0 : s0 = t0) : unfold m_Val s0 = unfold m_Val t0.
 Proof.
 exact (eq_trans eq_refl (ap (fun x => unfold m_Val x) H0)).
-Qed.
-
-Lemma congr_box {m_Val : nat} {s0 : Val m_Val} {t0 : Val m_Val}
-  (H0 : s0 = t0) : box m_Val s0 = box m_Val t0.
-Proof.
-exact (eq_trans eq_refl (ap (fun x => box m_Val x) H0)).
-Qed.
-
-Lemma congr_bind {m_Val : nat} {s0 : Tm m_Val} {s1 : Tm (S m_Val)}
-  {t0 : Tm m_Val} {t1 : Tm (S m_Val)} (H0 : s0 = t0) (H1 : s1 = t1) :
-  bind m_Val s0 s1 = bind m_Val t0 t1.
-Proof.
-exact (eq_trans (eq_trans eq_refl (ap (fun x => bind m_Val x s1) H0))
-         (ap (fun x => bind m_Val t0 x) H1)).
 Qed.
 
 Lemma upRen_Val_Val {m : nat} {n : nat} (xi : fin m -> fin n) :
@@ -167,11 +148,12 @@ Fixpoint ren_Val {m_Val : nat} {n_Val : nat}
 (xi_Val : fin m_Val -> fin n_Val) (s : Val m_Val) {struct s} : Val n_Val :=
   match s with
   | var _ s0 => var n_Val (xi_Val s0)
+  | unit _ => unit n_Val
+  | abs _ s0 => abs n_Val (ren_Tm (upRen_Val_Val xi_Val) s0)
   | zero _ => zero n_Val
   | succ _ s0 => succ n_Val (ren_Val xi_Val s0)
   | prod _ s0 s1 => prod n_Val (ren_Val xi_Val s0) (ren_Val xi_Val s1)
   | inj _ s0 s1 => inj n_Val s0 (ren_Val xi_Val s1)
-  | abs _ s0 => abs n_Val (ren_Tm (upRen_Val_Val xi_Val) s0)
   | rec _ s0 => rec n_Val (ren_Val (upRen_Val_Val xi_Val) s0)
   | fold _ s0 => fold n_Val (ren_Val xi_Val s0)
   end
@@ -181,21 +163,15 @@ with ren_Tm {m_Val : nat} {n_Val : nat} (xi_Val : fin m_Val -> fin n_Val)
   | ret _ s0 => ret n_Val (ren_Val xi_Val s0)
   | let_ _ s0 s1 =>
       let_ n_Val (ren_Tm xi_Val s0) (ren_Tm (upRen_Val_Val xi_Val) s1)
+  | app _ s0 s1 => app n_Val (ren_Val xi_Val s0) (ren_Val xi_Val s1)
   | ifz _ s0 s1 s2 =>
       ifz n_Val (ren_Val xi_Val s0) (ren_Tm xi_Val s1)
         (ren_Tm (upRen_Val_Val xi_Val) s2)
   | prj _ s0 s1 => prj n_Val s0 (ren_Val xi_Val s1)
-  | split _ s0 s1 =>
-      split n_Val (ren_Val xi_Val s0)
-        (ren_Tm (upRen_Val_Val (upRen_Val_Val xi_Val)) s1)
   | case _ s0 s1 s2 =>
       case n_Val (ren_Val xi_Val s0) (ren_Tm (upRen_Val_Val xi_Val) s1)
         (ren_Tm (upRen_Val_Val xi_Val) s2)
-  | app _ s0 s1 => app n_Val (ren_Val xi_Val s0) (ren_Val xi_Val s1)
   | unfold _ s0 => unfold n_Val (ren_Val xi_Val s0)
-  | box _ s0 => box n_Val (ren_Val xi_Val s0)
-  | bind _ s0 s1 =>
-      bind n_Val (ren_Tm xi_Val s0) (ren_Tm (upRen_Val_Val xi_Val) s1)
   end.
 
 Lemma up_Val_Val {m : nat} {n_Val : nat} (sigma : fin m -> Val n_Val) :
@@ -216,12 +192,13 @@ Fixpoint subst_Val {m_Val : nat} {n_Val : nat}
 :=
   match s with
   | var _ s0 => sigma_Val s0
+  | unit _ => unit n_Val
+  | abs _ s0 => abs n_Val (subst_Tm (up_Val_Val sigma_Val) s0)
   | zero _ => zero n_Val
   | succ _ s0 => succ n_Val (subst_Val sigma_Val s0)
   | prod _ s0 s1 =>
       prod n_Val (subst_Val sigma_Val s0) (subst_Val sigma_Val s1)
   | inj _ s0 s1 => inj n_Val s0 (subst_Val sigma_Val s1)
-  | abs _ s0 => abs n_Val (subst_Tm (up_Val_Val sigma_Val) s0)
   | rec _ s0 => rec n_Val (subst_Val (up_Val_Val sigma_Val) s0)
   | fold _ s0 => fold n_Val (subst_Val sigma_Val s0)
   end
@@ -231,23 +208,17 @@ with subst_Tm {m_Val : nat} {n_Val : nat}
   | ret _ s0 => ret n_Val (subst_Val sigma_Val s0)
   | let_ _ s0 s1 =>
       let_ n_Val (subst_Tm sigma_Val s0) (subst_Tm (up_Val_Val sigma_Val) s1)
+  | app _ s0 s1 =>
+      app n_Val (subst_Val sigma_Val s0) (subst_Val sigma_Val s1)
   | ifz _ s0 s1 s2 =>
       ifz n_Val (subst_Val sigma_Val s0) (subst_Tm sigma_Val s1)
         (subst_Tm (up_Val_Val sigma_Val) s2)
   | prj _ s0 s1 => prj n_Val s0 (subst_Val sigma_Val s1)
-  | split _ s0 s1 =>
-      split n_Val (subst_Val sigma_Val s0)
-        (subst_Tm (up_Val_Val (up_Val_Val sigma_Val)) s1)
   | case _ s0 s1 s2 =>
       case n_Val (subst_Val sigma_Val s0)
         (subst_Tm (up_Val_Val sigma_Val) s1)
         (subst_Tm (up_Val_Val sigma_Val) s2)
-  | app _ s0 s1 =>
-      app n_Val (subst_Val sigma_Val s0) (subst_Val sigma_Val s1)
   | unfold _ s0 => unfold n_Val (subst_Val sigma_Val s0)
-  | box _ s0 => box n_Val (subst_Val sigma_Val s0)
-  | bind _ s0 s1 =>
-      bind n_Val (subst_Tm sigma_Val s0) (subst_Tm (up_Val_Val sigma_Val) s1)
   end.
 
 Lemma upId_Val_Val {m_Val : nat} (sigma : fin m_Val -> Val m_Val)
@@ -275,15 +246,16 @@ Fixpoint idSubst_Val {m_Val : nat} (sigma_Val : fin m_Val -> Val m_Val)
 subst_Val sigma_Val s = s :=
   match s with
   | var _ s0 => Eq_Val s0
+  | unit _ => congr_unit
+  | abs _ s0 =>
+      congr_abs
+        (idSubst_Tm (up_Val_Val sigma_Val) (upId_Val_Val _ Eq_Val) s0)
   | zero _ => congr_zero
   | succ _ s0 => congr_succ (idSubst_Val sigma_Val Eq_Val s0)
   | prod _ s0 s1 =>
       congr_prod (idSubst_Val sigma_Val Eq_Val s0)
         (idSubst_Val sigma_Val Eq_Val s1)
   | inj _ s0 s1 => congr_inj (eq_refl s0) (idSubst_Val sigma_Val Eq_Val s1)
-  | abs _ s0 =>
-      congr_abs
-        (idSubst_Tm (up_Val_Val sigma_Val) (upId_Val_Val _ Eq_Val) s0)
   | rec _ s0 =>
       congr_rec
         (idSubst_Val (up_Val_Val sigma_Val) (upId_Val_Val _ Eq_Val) s0)
@@ -297,27 +269,19 @@ subst_Tm sigma_Val s = s :=
   | let_ _ s0 s1 =>
       congr_let_ (idSubst_Tm sigma_Val Eq_Val s0)
         (idSubst_Tm (up_Val_Val sigma_Val) (upId_Val_Val _ Eq_Val) s1)
+  | app _ s0 s1 =>
+      congr_app (idSubst_Val sigma_Val Eq_Val s0)
+        (idSubst_Val sigma_Val Eq_Val s1)
   | ifz _ s0 s1 s2 =>
       congr_ifz (idSubst_Val sigma_Val Eq_Val s0)
         (idSubst_Tm sigma_Val Eq_Val s1)
         (idSubst_Tm (up_Val_Val sigma_Val) (upId_Val_Val _ Eq_Val) s2)
   | prj _ s0 s1 => congr_prj (eq_refl s0) (idSubst_Val sigma_Val Eq_Val s1)
-  | split _ s0 s1 =>
-      congr_split (idSubst_Val sigma_Val Eq_Val s0)
-        (idSubst_Tm (up_Val_Val (up_Val_Val sigma_Val))
-           (upId_Val_Val _ (upId_Val_Val _ Eq_Val)) s1)
   | case _ s0 s1 s2 =>
       congr_case (idSubst_Val sigma_Val Eq_Val s0)
         (idSubst_Tm (up_Val_Val sigma_Val) (upId_Val_Val _ Eq_Val) s1)
         (idSubst_Tm (up_Val_Val sigma_Val) (upId_Val_Val _ Eq_Val) s2)
-  | app _ s0 s1 =>
-      congr_app (idSubst_Val sigma_Val Eq_Val s0)
-        (idSubst_Val sigma_Val Eq_Val s1)
   | unfold _ s0 => congr_unfold (idSubst_Val sigma_Val Eq_Val s0)
-  | box _ s0 => congr_box (idSubst_Val sigma_Val Eq_Val s0)
-  | bind _ s0 s1 =>
-      congr_bind (idSubst_Tm sigma_Val Eq_Val s0)
-        (idSubst_Tm (up_Val_Val sigma_Val) (upId_Val_Val _ Eq_Val) s1)
   end.
 
 Lemma upExtRen_Val_Val {m : nat} {n : nat} (xi : fin m -> fin n)
@@ -346,6 +310,11 @@ Fixpoint extRen_Val {m_Val : nat} {n_Val : nat}
 ren_Val xi_Val s = ren_Val zeta_Val s :=
   match s with
   | var _ s0 => ap (var n_Val) (Eq_Val s0)
+  | unit _ => congr_unit
+  | abs _ s0 =>
+      congr_abs
+        (extRen_Tm (upRen_Val_Val xi_Val) (upRen_Val_Val zeta_Val)
+           (upExtRen_Val_Val _ _ Eq_Val) s0)
   | zero _ => congr_zero
   | succ _ s0 => congr_succ (extRen_Val xi_Val zeta_Val Eq_Val s0)
   | prod _ s0 s1 =>
@@ -353,10 +322,6 @@ ren_Val xi_Val s = ren_Val zeta_Val s :=
         (extRen_Val xi_Val zeta_Val Eq_Val s1)
   | inj _ s0 s1 =>
       congr_inj (eq_refl s0) (extRen_Val xi_Val zeta_Val Eq_Val s1)
-  | abs _ s0 =>
-      congr_abs
-        (extRen_Tm (upRen_Val_Val xi_Val) (upRen_Val_Val zeta_Val)
-           (upExtRen_Val_Val _ _ Eq_Val) s0)
   | rec _ s0 =>
       congr_rec
         (extRen_Val (upRen_Val_Val xi_Val) (upRen_Val_Val zeta_Val)
@@ -373,6 +338,9 @@ ren_Tm xi_Val s = ren_Tm zeta_Val s :=
       congr_let_ (extRen_Tm xi_Val zeta_Val Eq_Val s0)
         (extRen_Tm (upRen_Val_Val xi_Val) (upRen_Val_Val zeta_Val)
            (upExtRen_Val_Val _ _ Eq_Val) s1)
+  | app _ s0 s1 =>
+      congr_app (extRen_Val xi_Val zeta_Val Eq_Val s0)
+        (extRen_Val xi_Val zeta_Val Eq_Val s1)
   | ifz _ s0 s1 s2 =>
       congr_ifz (extRen_Val xi_Val zeta_Val Eq_Val s0)
         (extRen_Tm xi_Val zeta_Val Eq_Val s1)
@@ -380,26 +348,13 @@ ren_Tm xi_Val s = ren_Tm zeta_Val s :=
            (upExtRen_Val_Val _ _ Eq_Val) s2)
   | prj _ s0 s1 =>
       congr_prj (eq_refl s0) (extRen_Val xi_Val zeta_Val Eq_Val s1)
-  | split _ s0 s1 =>
-      congr_split (extRen_Val xi_Val zeta_Val Eq_Val s0)
-        (extRen_Tm (upRen_Val_Val (upRen_Val_Val xi_Val))
-           (upRen_Val_Val (upRen_Val_Val zeta_Val))
-           (upExtRen_Val_Val _ _ (upExtRen_Val_Val _ _ Eq_Val)) s1)
   | case _ s0 s1 s2 =>
       congr_case (extRen_Val xi_Val zeta_Val Eq_Val s0)
         (extRen_Tm (upRen_Val_Val xi_Val) (upRen_Val_Val zeta_Val)
            (upExtRen_Val_Val _ _ Eq_Val) s1)
         (extRen_Tm (upRen_Val_Val xi_Val) (upRen_Val_Val zeta_Val)
            (upExtRen_Val_Val _ _ Eq_Val) s2)
-  | app _ s0 s1 =>
-      congr_app (extRen_Val xi_Val zeta_Val Eq_Val s0)
-        (extRen_Val xi_Val zeta_Val Eq_Val s1)
   | unfold _ s0 => congr_unfold (extRen_Val xi_Val zeta_Val Eq_Val s0)
-  | box _ s0 => congr_box (extRen_Val xi_Val zeta_Val Eq_Val s0)
-  | bind _ s0 s1 =>
-      congr_bind (extRen_Tm xi_Val zeta_Val Eq_Val s0)
-        (extRen_Tm (upRen_Val_Val xi_Val) (upRen_Val_Val zeta_Val)
-           (upExtRen_Val_Val _ _ Eq_Val) s1)
   end.
 
 Lemma upExt_Val_Val {m : nat} {n_Val : nat} (sigma : fin m -> Val n_Val)
@@ -429,6 +384,11 @@ Fixpoint ext_Val {m_Val : nat} {n_Val : nat}
 subst_Val sigma_Val s = subst_Val tau_Val s :=
   match s with
   | var _ s0 => Eq_Val s0
+  | unit _ => congr_unit
+  | abs _ s0 =>
+      congr_abs
+        (ext_Tm (up_Val_Val sigma_Val) (up_Val_Val tau_Val)
+           (upExt_Val_Val _ _ Eq_Val) s0)
   | zero _ => congr_zero
   | succ _ s0 => congr_succ (ext_Val sigma_Val tau_Val Eq_Val s0)
   | prod _ s0 s1 =>
@@ -436,10 +396,6 @@ subst_Val sigma_Val s = subst_Val tau_Val s :=
         (ext_Val sigma_Val tau_Val Eq_Val s1)
   | inj _ s0 s1 =>
       congr_inj (eq_refl s0) (ext_Val sigma_Val tau_Val Eq_Val s1)
-  | abs _ s0 =>
-      congr_abs
-        (ext_Tm (up_Val_Val sigma_Val) (up_Val_Val tau_Val)
-           (upExt_Val_Val _ _ Eq_Val) s0)
   | rec _ s0 =>
       congr_rec
         (ext_Val (up_Val_Val sigma_Val) (up_Val_Val tau_Val)
@@ -456,6 +412,9 @@ subst_Tm sigma_Val s = subst_Tm tau_Val s :=
       congr_let_ (ext_Tm sigma_Val tau_Val Eq_Val s0)
         (ext_Tm (up_Val_Val sigma_Val) (up_Val_Val tau_Val)
            (upExt_Val_Val _ _ Eq_Val) s1)
+  | app _ s0 s1 =>
+      congr_app (ext_Val sigma_Val tau_Val Eq_Val s0)
+        (ext_Val sigma_Val tau_Val Eq_Val s1)
   | ifz _ s0 s1 s2 =>
       congr_ifz (ext_Val sigma_Val tau_Val Eq_Val s0)
         (ext_Tm sigma_Val tau_Val Eq_Val s1)
@@ -463,26 +422,13 @@ subst_Tm sigma_Val s = subst_Tm tau_Val s :=
            (upExt_Val_Val _ _ Eq_Val) s2)
   | prj _ s0 s1 =>
       congr_prj (eq_refl s0) (ext_Val sigma_Val tau_Val Eq_Val s1)
-  | split _ s0 s1 =>
-      congr_split (ext_Val sigma_Val tau_Val Eq_Val s0)
-        (ext_Tm (up_Val_Val (up_Val_Val sigma_Val))
-           (up_Val_Val (up_Val_Val tau_Val))
-           (upExt_Val_Val _ _ (upExt_Val_Val _ _ Eq_Val)) s1)
   | case _ s0 s1 s2 =>
       congr_case (ext_Val sigma_Val tau_Val Eq_Val s0)
         (ext_Tm (up_Val_Val sigma_Val) (up_Val_Val tau_Val)
            (upExt_Val_Val _ _ Eq_Val) s1)
         (ext_Tm (up_Val_Val sigma_Val) (up_Val_Val tau_Val)
            (upExt_Val_Val _ _ Eq_Val) s2)
-  | app _ s0 s1 =>
-      congr_app (ext_Val sigma_Val tau_Val Eq_Val s0)
-        (ext_Val sigma_Val tau_Val Eq_Val s1)
   | unfold _ s0 => congr_unfold (ext_Val sigma_Val tau_Val Eq_Val s0)
-  | box _ s0 => congr_box (ext_Val sigma_Val tau_Val Eq_Val s0)
-  | bind _ s0 s1 =>
-      congr_bind (ext_Tm sigma_Val tau_Val Eq_Val s0)
-        (ext_Tm (up_Val_Val sigma_Val) (up_Val_Val tau_Val)
-           (upExt_Val_Val _ _ Eq_Val) s1)
   end.
 
 Lemma up_ren_ren_Val_Val {k : nat} {l : nat} {m : nat} (xi : fin k -> fin l)
@@ -511,6 +457,11 @@ Fixpoint compRenRen_Val {k_Val : nat} {l_Val : nat} {m_Val : nat}
 {struct s} : ren_Val zeta_Val (ren_Val xi_Val s) = ren_Val rho_Val s :=
   match s with
   | var _ s0 => ap (var l_Val) (Eq_Val s0)
+  | unit _ => congr_unit
+  | abs _ s0 =>
+      congr_abs
+        (compRenRen_Tm (upRen_Val_Val xi_Val) (upRen_Val_Val zeta_Val)
+           (upRen_Val_Val rho_Val) (up_ren_ren _ _ _ Eq_Val) s0)
   | zero _ => congr_zero
   | succ _ s0 =>
       congr_succ (compRenRen_Val xi_Val zeta_Val rho_Val Eq_Val s0)
@@ -520,10 +471,6 @@ Fixpoint compRenRen_Val {k_Val : nat} {l_Val : nat} {m_Val : nat}
   | inj _ s0 s1 =>
       congr_inj (eq_refl s0)
         (compRenRen_Val xi_Val zeta_Val rho_Val Eq_Val s1)
-  | abs _ s0 =>
-      congr_abs
-        (compRenRen_Tm (upRen_Val_Val xi_Val) (upRen_Val_Val zeta_Val)
-           (upRen_Val_Val rho_Val) (up_ren_ren _ _ _ Eq_Val) s0)
   | rec _ s0 =>
       congr_rec
         (compRenRen_Val (upRen_Val_Val xi_Val) (upRen_Val_Val zeta_Val)
@@ -542,6 +489,9 @@ with compRenRen_Tm {k_Val : nat} {l_Val : nat} {m_Val : nat}
       congr_let_ (compRenRen_Tm xi_Val zeta_Val rho_Val Eq_Val s0)
         (compRenRen_Tm (upRen_Val_Val xi_Val) (upRen_Val_Val zeta_Val)
            (upRen_Val_Val rho_Val) (up_ren_ren _ _ _ Eq_Val) s1)
+  | app _ s0 s1 =>
+      congr_app (compRenRen_Val xi_Val zeta_Val rho_Val Eq_Val s0)
+        (compRenRen_Val xi_Val zeta_Val rho_Val Eq_Val s1)
   | ifz _ s0 s1 s2 =>
       congr_ifz (compRenRen_Val xi_Val zeta_Val rho_Val Eq_Val s0)
         (compRenRen_Tm xi_Val zeta_Val rho_Val Eq_Val s1)
@@ -550,28 +500,14 @@ with compRenRen_Tm {k_Val : nat} {l_Val : nat} {m_Val : nat}
   | prj _ s0 s1 =>
       congr_prj (eq_refl s0)
         (compRenRen_Val xi_Val zeta_Val rho_Val Eq_Val s1)
-  | split _ s0 s1 =>
-      congr_split (compRenRen_Val xi_Val zeta_Val rho_Val Eq_Val s0)
-        (compRenRen_Tm (upRen_Val_Val (upRen_Val_Val xi_Val))
-           (upRen_Val_Val (upRen_Val_Val zeta_Val))
-           (upRen_Val_Val (upRen_Val_Val rho_Val))
-           (up_ren_ren _ _ _ (up_ren_ren _ _ _ Eq_Val)) s1)
   | case _ s0 s1 s2 =>
       congr_case (compRenRen_Val xi_Val zeta_Val rho_Val Eq_Val s0)
         (compRenRen_Tm (upRen_Val_Val xi_Val) (upRen_Val_Val zeta_Val)
            (upRen_Val_Val rho_Val) (up_ren_ren _ _ _ Eq_Val) s1)
         (compRenRen_Tm (upRen_Val_Val xi_Val) (upRen_Val_Val zeta_Val)
            (upRen_Val_Val rho_Val) (up_ren_ren _ _ _ Eq_Val) s2)
-  | app _ s0 s1 =>
-      congr_app (compRenRen_Val xi_Val zeta_Val rho_Val Eq_Val s0)
-        (compRenRen_Val xi_Val zeta_Val rho_Val Eq_Val s1)
   | unfold _ s0 =>
       congr_unfold (compRenRen_Val xi_Val zeta_Val rho_Val Eq_Val s0)
-  | box _ s0 => congr_box (compRenRen_Val xi_Val zeta_Val rho_Val Eq_Val s0)
-  | bind _ s0 s1 =>
-      congr_bind (compRenRen_Tm xi_Val zeta_Val rho_Val Eq_Val s0)
-        (compRenRen_Tm (upRen_Val_Val xi_Val) (upRen_Val_Val zeta_Val)
-           (upRen_Val_Val rho_Val) (up_ren_ren _ _ _ Eq_Val) s1)
   end.
 
 Lemma up_ren_subst_Val_Val {k : nat} {l : nat} {m_Val : nat}
@@ -609,6 +545,11 @@ Fixpoint compRenSubst_Val {k_Val : nat} {l_Val : nat} {m_Val : nat}
 {struct s} : subst_Val tau_Val (ren_Val xi_Val s) = subst_Val theta_Val s :=
   match s with
   | var _ s0 => Eq_Val s0
+  | unit _ => congr_unit
+  | abs _ s0 =>
+      congr_abs
+        (compRenSubst_Tm (upRen_Val_Val xi_Val) (up_Val_Val tau_Val)
+           (up_Val_Val theta_Val) (up_ren_subst_Val_Val _ _ _ Eq_Val) s0)
   | zero _ => congr_zero
   | succ _ s0 =>
       congr_succ (compRenSubst_Val xi_Val tau_Val theta_Val Eq_Val s0)
@@ -618,10 +559,6 @@ Fixpoint compRenSubst_Val {k_Val : nat} {l_Val : nat} {m_Val : nat}
   | inj _ s0 s1 =>
       congr_inj (eq_refl s0)
         (compRenSubst_Val xi_Val tau_Val theta_Val Eq_Val s1)
-  | abs _ s0 =>
-      congr_abs
-        (compRenSubst_Tm (upRen_Val_Val xi_Val) (up_Val_Val tau_Val)
-           (up_Val_Val theta_Val) (up_ren_subst_Val_Val _ _ _ Eq_Val) s0)
   | rec _ s0 =>
       congr_rec
         (compRenSubst_Val (upRen_Val_Val xi_Val) (up_Val_Val tau_Val)
@@ -641,6 +578,9 @@ with compRenSubst_Tm {k_Val : nat} {l_Val : nat} {m_Val : nat}
       congr_let_ (compRenSubst_Tm xi_Val tau_Val theta_Val Eq_Val s0)
         (compRenSubst_Tm (upRen_Val_Val xi_Val) (up_Val_Val tau_Val)
            (up_Val_Val theta_Val) (up_ren_subst_Val_Val _ _ _ Eq_Val) s1)
+  | app _ s0 s1 =>
+      congr_app (compRenSubst_Val xi_Val tau_Val theta_Val Eq_Val s0)
+        (compRenSubst_Val xi_Val tau_Val theta_Val Eq_Val s1)
   | ifz _ s0 s1 s2 =>
       congr_ifz (compRenSubst_Val xi_Val tau_Val theta_Val Eq_Val s0)
         (compRenSubst_Tm xi_Val tau_Val theta_Val Eq_Val s1)
@@ -649,30 +589,14 @@ with compRenSubst_Tm {k_Val : nat} {l_Val : nat} {m_Val : nat}
   | prj _ s0 s1 =>
       congr_prj (eq_refl s0)
         (compRenSubst_Val xi_Val tau_Val theta_Val Eq_Val s1)
-  | split _ s0 s1 =>
-      congr_split (compRenSubst_Val xi_Val tau_Val theta_Val Eq_Val s0)
-        (compRenSubst_Tm (upRen_Val_Val (upRen_Val_Val xi_Val))
-           (up_Val_Val (up_Val_Val tau_Val))
-           (up_Val_Val (up_Val_Val theta_Val))
-           (up_ren_subst_Val_Val _ _ _ (up_ren_subst_Val_Val _ _ _ Eq_Val))
-           s1)
   | case _ s0 s1 s2 =>
       congr_case (compRenSubst_Val xi_Val tau_Val theta_Val Eq_Val s0)
         (compRenSubst_Tm (upRen_Val_Val xi_Val) (up_Val_Val tau_Val)
            (up_Val_Val theta_Val) (up_ren_subst_Val_Val _ _ _ Eq_Val) s1)
         (compRenSubst_Tm (upRen_Val_Val xi_Val) (up_Val_Val tau_Val)
            (up_Val_Val theta_Val) (up_ren_subst_Val_Val _ _ _ Eq_Val) s2)
-  | app _ s0 s1 =>
-      congr_app (compRenSubst_Val xi_Val tau_Val theta_Val Eq_Val s0)
-        (compRenSubst_Val xi_Val tau_Val theta_Val Eq_Val s1)
   | unfold _ s0 =>
       congr_unfold (compRenSubst_Val xi_Val tau_Val theta_Val Eq_Val s0)
-  | box _ s0 =>
-      congr_box (compRenSubst_Val xi_Val tau_Val theta_Val Eq_Val s0)
-  | bind _ s0 s1 =>
-      congr_bind (compRenSubst_Tm xi_Val tau_Val theta_Val Eq_Val s0)
-        (compRenSubst_Tm (upRen_Val_Val xi_Val) (up_Val_Val tau_Val)
-           (up_Val_Val theta_Val) (up_ren_subst_Val_Val _ _ _ Eq_Val) s1)
   end.
 
 Lemma up_subst_ren_Val_Val {k : nat} {l_Val : nat} {m_Val : nat}
@@ -732,6 +656,11 @@ Fixpoint compSubstRen_Val {k_Val : nat} {l_Val : nat} {m_Val : nat}
 ren_Val zeta_Val (subst_Val sigma_Val s) = subst_Val theta_Val s :=
   match s with
   | var _ s0 => Eq_Val s0
+  | unit _ => congr_unit
+  | abs _ s0 =>
+      congr_abs
+        (compSubstRen_Tm (up_Val_Val sigma_Val) (upRen_Val_Val zeta_Val)
+           (up_Val_Val theta_Val) (up_subst_ren_Val_Val _ _ _ Eq_Val) s0)
   | zero _ => congr_zero
   | succ _ s0 =>
       congr_succ (compSubstRen_Val sigma_Val zeta_Val theta_Val Eq_Val s0)
@@ -741,10 +670,6 @@ ren_Val zeta_Val (subst_Val sigma_Val s) = subst_Val theta_Val s :=
   | inj _ s0 s1 =>
       congr_inj (eq_refl s0)
         (compSubstRen_Val sigma_Val zeta_Val theta_Val Eq_Val s1)
-  | abs _ s0 =>
-      congr_abs
-        (compSubstRen_Tm (up_Val_Val sigma_Val) (upRen_Val_Val zeta_Val)
-           (up_Val_Val theta_Val) (up_subst_ren_Val_Val _ _ _ Eq_Val) s0)
   | rec _ s0 =>
       congr_rec
         (compSubstRen_Val (up_Val_Val sigma_Val) (upRen_Val_Val zeta_Val)
@@ -765,6 +690,9 @@ ren_Tm zeta_Val (subst_Tm sigma_Val s) = subst_Tm theta_Val s :=
       congr_let_ (compSubstRen_Tm sigma_Val zeta_Val theta_Val Eq_Val s0)
         (compSubstRen_Tm (up_Val_Val sigma_Val) (upRen_Val_Val zeta_Val)
            (up_Val_Val theta_Val) (up_subst_ren_Val_Val _ _ _ Eq_Val) s1)
+  | app _ s0 s1 =>
+      congr_app (compSubstRen_Val sigma_Val zeta_Val theta_Val Eq_Val s0)
+        (compSubstRen_Val sigma_Val zeta_Val theta_Val Eq_Val s1)
   | ifz _ s0 s1 s2 =>
       congr_ifz (compSubstRen_Val sigma_Val zeta_Val theta_Val Eq_Val s0)
         (compSubstRen_Tm sigma_Val zeta_Val theta_Val Eq_Val s1)
@@ -773,30 +701,14 @@ ren_Tm zeta_Val (subst_Tm sigma_Val s) = subst_Tm theta_Val s :=
   | prj _ s0 s1 =>
       congr_prj (eq_refl s0)
         (compSubstRen_Val sigma_Val zeta_Val theta_Val Eq_Val s1)
-  | split _ s0 s1 =>
-      congr_split (compSubstRen_Val sigma_Val zeta_Val theta_Val Eq_Val s0)
-        (compSubstRen_Tm (up_Val_Val (up_Val_Val sigma_Val))
-           (upRen_Val_Val (upRen_Val_Val zeta_Val))
-           (up_Val_Val (up_Val_Val theta_Val))
-           (up_subst_ren_Val_Val _ _ _ (up_subst_ren_Val_Val _ _ _ Eq_Val))
-           s1)
   | case _ s0 s1 s2 =>
       congr_case (compSubstRen_Val sigma_Val zeta_Val theta_Val Eq_Val s0)
         (compSubstRen_Tm (up_Val_Val sigma_Val) (upRen_Val_Val zeta_Val)
            (up_Val_Val theta_Val) (up_subst_ren_Val_Val _ _ _ Eq_Val) s1)
         (compSubstRen_Tm (up_Val_Val sigma_Val) (upRen_Val_Val zeta_Val)
            (up_Val_Val theta_Val) (up_subst_ren_Val_Val _ _ _ Eq_Val) s2)
-  | app _ s0 s1 =>
-      congr_app (compSubstRen_Val sigma_Val zeta_Val theta_Val Eq_Val s0)
-        (compSubstRen_Val sigma_Val zeta_Val theta_Val Eq_Val s1)
   | unfold _ s0 =>
       congr_unfold (compSubstRen_Val sigma_Val zeta_Val theta_Val Eq_Val s0)
-  | box _ s0 =>
-      congr_box (compSubstRen_Val sigma_Val zeta_Val theta_Val Eq_Val s0)
-  | bind _ s0 s1 =>
-      congr_bind (compSubstRen_Tm sigma_Val zeta_Val theta_Val Eq_Val s0)
-        (compSubstRen_Tm (up_Val_Val sigma_Val) (upRen_Val_Val zeta_Val)
-           (up_Val_Val theta_Val) (up_subst_ren_Val_Val _ _ _ Eq_Val) s1)
   end.
 
 Lemma up_subst_subst_Val_Val {k : nat} {l_Val : nat} {m_Val : nat}
@@ -857,6 +769,11 @@ Fixpoint compSubstSubst_Val {k_Val : nat} {l_Val : nat} {m_Val : nat}
 subst_Val tau_Val (subst_Val sigma_Val s) = subst_Val theta_Val s :=
   match s with
   | var _ s0 => Eq_Val s0
+  | unit _ => congr_unit
+  | abs _ s0 =>
+      congr_abs
+        (compSubstSubst_Tm (up_Val_Val sigma_Val) (up_Val_Val tau_Val)
+           (up_Val_Val theta_Val) (up_subst_subst_Val_Val _ _ _ Eq_Val) s0)
   | zero _ => congr_zero
   | succ _ s0 =>
       congr_succ (compSubstSubst_Val sigma_Val tau_Val theta_Val Eq_Val s0)
@@ -866,10 +783,6 @@ subst_Val tau_Val (subst_Val sigma_Val s) = subst_Val theta_Val s :=
   | inj _ s0 s1 =>
       congr_inj (eq_refl s0)
         (compSubstSubst_Val sigma_Val tau_Val theta_Val Eq_Val s1)
-  | abs _ s0 =>
-      congr_abs
-        (compSubstSubst_Tm (up_Val_Val sigma_Val) (up_Val_Val tau_Val)
-           (up_Val_Val theta_Val) (up_subst_subst_Val_Val _ _ _ Eq_Val) s0)
   | rec _ s0 =>
       congr_rec
         (compSubstSubst_Val (up_Val_Val sigma_Val) (up_Val_Val tau_Val)
@@ -890,6 +803,9 @@ subst_Tm tau_Val (subst_Tm sigma_Val s) = subst_Tm theta_Val s :=
       congr_let_ (compSubstSubst_Tm sigma_Val tau_Val theta_Val Eq_Val s0)
         (compSubstSubst_Tm (up_Val_Val sigma_Val) (up_Val_Val tau_Val)
            (up_Val_Val theta_Val) (up_subst_subst_Val_Val _ _ _ Eq_Val) s1)
+  | app _ s0 s1 =>
+      congr_app (compSubstSubst_Val sigma_Val tau_Val theta_Val Eq_Val s0)
+        (compSubstSubst_Val sigma_Val tau_Val theta_Val Eq_Val s1)
   | ifz _ s0 s1 s2 =>
       congr_ifz (compSubstSubst_Val sigma_Val tau_Val theta_Val Eq_Val s0)
         (compSubstSubst_Tm sigma_Val tau_Val theta_Val Eq_Val s1)
@@ -898,31 +814,14 @@ subst_Tm tau_Val (subst_Tm sigma_Val s) = subst_Tm theta_Val s :=
   | prj _ s0 s1 =>
       congr_prj (eq_refl s0)
         (compSubstSubst_Val sigma_Val tau_Val theta_Val Eq_Val s1)
-  | split _ s0 s1 =>
-      congr_split (compSubstSubst_Val sigma_Val tau_Val theta_Val Eq_Val s0)
-        (compSubstSubst_Tm (up_Val_Val (up_Val_Val sigma_Val))
-           (up_Val_Val (up_Val_Val tau_Val))
-           (up_Val_Val (up_Val_Val theta_Val))
-           (up_subst_subst_Val_Val _ _ _
-              (up_subst_subst_Val_Val _ _ _ Eq_Val))
-           s1)
   | case _ s0 s1 s2 =>
       congr_case (compSubstSubst_Val sigma_Val tau_Val theta_Val Eq_Val s0)
         (compSubstSubst_Tm (up_Val_Val sigma_Val) (up_Val_Val tau_Val)
            (up_Val_Val theta_Val) (up_subst_subst_Val_Val _ _ _ Eq_Val) s1)
         (compSubstSubst_Tm (up_Val_Val sigma_Val) (up_Val_Val tau_Val)
            (up_Val_Val theta_Val) (up_subst_subst_Val_Val _ _ _ Eq_Val) s2)
-  | app _ s0 s1 =>
-      congr_app (compSubstSubst_Val sigma_Val tau_Val theta_Val Eq_Val s0)
-        (compSubstSubst_Val sigma_Val tau_Val theta_Val Eq_Val s1)
   | unfold _ s0 =>
       congr_unfold (compSubstSubst_Val sigma_Val tau_Val theta_Val Eq_Val s0)
-  | box _ s0 =>
-      congr_box (compSubstSubst_Val sigma_Val tau_Val theta_Val Eq_Val s0)
-  | bind _ s0 s1 =>
-      congr_bind (compSubstSubst_Tm sigma_Val tau_Val theta_Val Eq_Val s0)
-        (compSubstSubst_Tm (up_Val_Val sigma_Val) (up_Val_Val tau_Val)
-           (up_Val_Val theta_Val) (up_subst_subst_Val_Val _ _ _ Eq_Val) s1)
   end.
 
 Lemma renRen_Val {k_Val : nat} {l_Val : nat} {m_Val : nat}
@@ -1088,6 +987,11 @@ Fixpoint rinst_inst_Val {m_Val : nat} {n_Val : nat}
 (s : Val m_Val) {struct s} : ren_Val xi_Val s = subst_Val sigma_Val s :=
   match s with
   | var _ s0 => Eq_Val s0
+  | unit _ => congr_unit
+  | abs _ s0 =>
+      congr_abs
+        (rinst_inst_Tm (upRen_Val_Val xi_Val) (up_Val_Val sigma_Val)
+           (rinstInst_up_Val_Val _ _ Eq_Val) s0)
   | zero _ => congr_zero
   | succ _ s0 => congr_succ (rinst_inst_Val xi_Val sigma_Val Eq_Val s0)
   | prod _ s0 s1 =>
@@ -1095,10 +999,6 @@ Fixpoint rinst_inst_Val {m_Val : nat} {n_Val : nat}
         (rinst_inst_Val xi_Val sigma_Val Eq_Val s1)
   | inj _ s0 s1 =>
       congr_inj (eq_refl s0) (rinst_inst_Val xi_Val sigma_Val Eq_Val s1)
-  | abs _ s0 =>
-      congr_abs
-        (rinst_inst_Tm (upRen_Val_Val xi_Val) (up_Val_Val sigma_Val)
-           (rinstInst_up_Val_Val _ _ Eq_Val) s0)
   | rec _ s0 =>
       congr_rec
         (rinst_inst_Val (upRen_Val_Val xi_Val) (up_Val_Val sigma_Val)
@@ -1115,6 +1015,9 @@ with rinst_inst_Tm {m_Val : nat} {n_Val : nat}
       congr_let_ (rinst_inst_Tm xi_Val sigma_Val Eq_Val s0)
         (rinst_inst_Tm (upRen_Val_Val xi_Val) (up_Val_Val sigma_Val)
            (rinstInst_up_Val_Val _ _ Eq_Val) s1)
+  | app _ s0 s1 =>
+      congr_app (rinst_inst_Val xi_Val sigma_Val Eq_Val s0)
+        (rinst_inst_Val xi_Val sigma_Val Eq_Val s1)
   | ifz _ s0 s1 s2 =>
       congr_ifz (rinst_inst_Val xi_Val sigma_Val Eq_Val s0)
         (rinst_inst_Tm xi_Val sigma_Val Eq_Val s1)
@@ -1122,26 +1025,13 @@ with rinst_inst_Tm {m_Val : nat} {n_Val : nat}
            (rinstInst_up_Val_Val _ _ Eq_Val) s2)
   | prj _ s0 s1 =>
       congr_prj (eq_refl s0) (rinst_inst_Val xi_Val sigma_Val Eq_Val s1)
-  | split _ s0 s1 =>
-      congr_split (rinst_inst_Val xi_Val sigma_Val Eq_Val s0)
-        (rinst_inst_Tm (upRen_Val_Val (upRen_Val_Val xi_Val))
-           (up_Val_Val (up_Val_Val sigma_Val))
-           (rinstInst_up_Val_Val _ _ (rinstInst_up_Val_Val _ _ Eq_Val)) s1)
   | case _ s0 s1 s2 =>
       congr_case (rinst_inst_Val xi_Val sigma_Val Eq_Val s0)
         (rinst_inst_Tm (upRen_Val_Val xi_Val) (up_Val_Val sigma_Val)
            (rinstInst_up_Val_Val _ _ Eq_Val) s1)
         (rinst_inst_Tm (upRen_Val_Val xi_Val) (up_Val_Val sigma_Val)
            (rinstInst_up_Val_Val _ _ Eq_Val) s2)
-  | app _ s0 s1 =>
-      congr_app (rinst_inst_Val xi_Val sigma_Val Eq_Val s0)
-        (rinst_inst_Val xi_Val sigma_Val Eq_Val s1)
   | unfold _ s0 => congr_unfold (rinst_inst_Val xi_Val sigma_Val Eq_Val s0)
-  | box _ s0 => congr_box (rinst_inst_Val xi_Val sigma_Val Eq_Val s0)
-  | bind _ s0 s1 =>
-      congr_bind (rinst_inst_Tm xi_Val sigma_Val Eq_Val s0)
-        (rinst_inst_Tm (upRen_Val_Val xi_Val) (up_Val_Val sigma_Val)
-           (rinstInst_up_Val_Val _ _ Eq_Val) s1)
   end.
 
 Lemma rinstInst'_Val {m_Val : nat} {n_Val : nat}
@@ -1249,11 +1139,96 @@ Proof.
 exact (fun x => eq_refl).
 Qed.
 
+Inductive Frame (n_Val : nat) : Type :=
+    f_let : Tm (S n_Val) -> Frame n_Val.
+
+Lemma congr_f_let {m_Val : nat} {s0 : Tm (S m_Val)} {t0 : Tm (S m_Val)}
+  (H0 : s0 = t0) : f_let m_Val s0 = f_let m_Val t0.
+Proof.
+exact (eq_trans eq_refl (ap (fun x => f_let m_Val x) H0)).
+Qed.
+
+Definition subst_Frame {m_Val : nat} {n_Val : nat}
+  (sigma_Val : fin m_Val -> Val n_Val) (s : Frame m_Val) : Frame n_Val :=
+  match s with
+  | f_let _ s0 => f_let n_Val (subst_Tm (up_Val_Val sigma_Val) s0)
+  end.
+
+Definition idSubst_Frame {m_Val : nat} (sigma_Val : fin m_Val -> Val m_Val)
+  (Eq_Val : forall x, sigma_Val x = var m_Val x) (s : Frame m_Val) :
+  subst_Frame sigma_Val s = s :=
+  match s with
+  | f_let _ s0 =>
+      congr_f_let
+        (idSubst_Tm (up_Val_Val sigma_Val) (upId_Val_Val _ Eq_Val) s0)
+  end.
+
+Definition ext_Frame {m_Val : nat} {n_Val : nat}
+  (sigma_Val : fin m_Val -> Val n_Val) (tau_Val : fin m_Val -> Val n_Val)
+  (Eq_Val : forall x, sigma_Val x = tau_Val x) (s : Frame m_Val) :
+  subst_Frame sigma_Val s = subst_Frame tau_Val s :=
+  match s with
+  | f_let _ s0 =>
+      congr_f_let
+        (ext_Tm (up_Val_Val sigma_Val) (up_Val_Val tau_Val)
+           (upExt_Val_Val _ _ Eq_Val) s0)
+  end.
+
+Definition compSubstSubst_Frame {k_Val : nat} {l_Val : nat} {m_Val : nat}
+  (sigma_Val : fin m_Val -> Val k_Val) (tau_Val : fin k_Val -> Val l_Val)
+  (theta_Val : fin m_Val -> Val l_Val)
+  (Eq_Val : forall x, funcomp (subst_Val tau_Val) sigma_Val x = theta_Val x)
+  (s : Frame m_Val) :
+  subst_Frame tau_Val (subst_Frame sigma_Val s) = subst_Frame theta_Val s :=
+  match s with
+  | f_let _ s0 =>
+      congr_f_let
+        (compSubstSubst_Tm (up_Val_Val sigma_Val) (up_Val_Val tau_Val)
+           (up_Val_Val theta_Val) (up_subst_subst_Val_Val _ _ _ Eq_Val) s0)
+  end.
+
+Lemma substSubst_Frame {k_Val : nat} {l_Val : nat} {m_Val : nat}
+  (sigma_Val : fin m_Val -> Val k_Val) (tau_Val : fin k_Val -> Val l_Val)
+  (s : Frame m_Val) :
+  subst_Frame tau_Val (subst_Frame sigma_Val s) =
+  subst_Frame (funcomp (subst_Val tau_Val) sigma_Val) s.
+Proof.
+exact (compSubstSubst_Frame sigma_Val tau_Val _ (fun n => eq_refl) s).
+Qed.
+
+Lemma substSubst_Frame_pointwise {k_Val : nat} {l_Val : nat} {m_Val : nat}
+  (sigma_Val : fin m_Val -> Val k_Val) (tau_Val : fin k_Val -> Val l_Val) :
+  pointwise_relation _ eq
+    (funcomp (subst_Frame tau_Val) (subst_Frame sigma_Val))
+    (subst_Frame (funcomp (subst_Val tau_Val) sigma_Val)).
+Proof.
+exact (fun s => compSubstSubst_Frame sigma_Val tau_Val _ (fun n => eq_refl) s).
+Qed.
+
+Lemma instId'_Frame {m_Val : nat} (s : Frame m_Val) :
+  subst_Frame (var m_Val) s = s.
+Proof.
+exact (idSubst_Frame (var m_Val) (fun n => eq_refl) s).
+Qed.
+
+Lemma instId'_Frame_pointwise {m_Val : nat} :
+  pointwise_relation _ eq (subst_Frame (var m_Val)) id.
+Proof.
+exact (fun s => idSubst_Frame (var m_Val) (fun n => eq_refl) s).
+Qed.
+
+Class Up_Frame X Y :=
+    up_Frame : X -> Y.
+
 Class Up_Tm X Y :=
     up_Tm : X -> Y.
 
 Class Up_Val X Y :=
     up_Val : X -> Y.
+
+#[global]
+Instance Subst_Frame  {m_Val n_Val : nat}: (Subst1 _ _ _) :=
+ (@subst_Frame m_Val n_Val).
 
 #[global]
 Instance Subst_Tm  {m_Val n_Val : nat}: (Subst1 _ _ _) :=
@@ -1274,6 +1249,11 @@ Instance Ren_Val  {m_Val n_Val : nat}: (Ren1 _ _ _) := (@ren_Val m_Val n_Val).
 
 #[global]
 Instance VarInstance_Val  {n_Val : nat}: (Var _ _) := (@var n_Val).
+
+Notation "s [ sigma_Val ]" := (subst_Frame sigma_Val s)
+( at level 7, left associativity, only printing)  : subst_scope.
+
+Notation "↑__Frame" := up_Frame (only printing)  : subst_scope.
 
 Notation "s [ sigma_Val ]" := (subst_Tm sigma_Val s)
 ( at level 7, left associativity, only printing)  : subst_scope.
@@ -1300,6 +1280,24 @@ Notation "x '__Val'" := (@ids _ _ VarInstance_Val x)
 
 Notation "x '__Val'" := (var x) ( at level 5, format "x __Val")  :
 subst_scope.
+
+#[global]
+Instance subst_Frame_morphism  {m_Val : nat} {n_Val : nat}:
+ (Proper (respectful (pointwise_relation _ eq) (respectful eq eq))
+    (@subst_Frame m_Val n_Val)).
+Proof.
+exact (fun f_Val g_Val Eq_Val s t Eq_st =>
+       eq_ind s (fun t' => subst_Frame f_Val s = subst_Frame g_Val t')
+         (ext_Frame f_Val g_Val Eq_Val s) t Eq_st).
+Qed.
+
+#[global]
+Instance subst_Frame_morphism2  {m_Val : nat} {n_Val : nat}:
+ (Proper (respectful (pointwise_relation _ eq) (pointwise_relation _ eq))
+    (@subst_Frame m_Val n_Val)).
+Proof.
+exact (fun f_Val g_Val Eq_Val s => ext_Frame f_Val g_Val Eq_Val s).
+Qed.
 
 #[global]
 Instance subst_Tm_morphism  {m_Val : nat} {n_Val : nat}:
@@ -1376,18 +1374,22 @@ Qed.
 Ltac auto_unfold := repeat
                      unfold VarInstance_Val, Var, ids, Ren_Val, Ren1, ren1,
                       Ren_Tm, Ren1, ren1, Up_Val_Val, Up_Val, up_Val,
-                      Subst_Val, Subst1, subst1, Subst_Tm, Subst1, subst1.
+                      Subst_Val, Subst1, subst1, Subst_Tm, Subst1, subst1,
+                      Subst_Frame, Subst1, subst1.
 
 Tactic Notation "auto_unfold" "in" "*" := repeat
                                            unfold VarInstance_Val, Var, ids,
                                             Ren_Val, Ren1, ren1, Ren_Tm,
                                             Ren1, ren1, Up_Val_Val, Up_Val,
                                             up_Val, Subst_Val, Subst1,
-                                            subst1, Subst_Tm, Subst1, subst1
+                                            subst1, Subst_Tm, Subst1, subst1,
+                                            Subst_Frame, Subst1, subst1 
                                             in *.
 
 Ltac asimpl' := repeat (first
-                 [ progress setoid_rewrite substSubst_Tm_pointwise
+                 [ progress setoid_rewrite substSubst_Frame_pointwise
+                 | progress setoid_rewrite substSubst_Frame
+                 | progress setoid_rewrite substSubst_Tm_pointwise
                  | progress setoid_rewrite substSubst_Tm
                  | progress setoid_rewrite substSubst_Val_pointwise
                  | progress setoid_rewrite substSubst_Val
@@ -1403,6 +1405,8 @@ Ltac asimpl' := repeat (first
                  | progress setoid_rewrite renRen_Tm
                  | progress setoid_rewrite renRen'_Val_pointwise
                  | progress setoid_rewrite renRen_Val
+                 | progress setoid_rewrite instId'_Frame_pointwise
+                 | progress setoid_rewrite instId'_Frame
                  | progress setoid_rewrite varLRen'_Val_pointwise
                  | progress setoid_rewrite varLRen'_Val
                  | progress setoid_rewrite varL'_Val_pointwise
@@ -1418,14 +1422,16 @@ Ltac asimpl' := repeat (first
                  | progress
                     unfold up_list_Val_Val, up_Val_Val, upRen_list_Val_Val,
                      upRen_Val_Val, up_ren
-                 | progress cbn[subst_Tm subst_Val ren_Tm ren_Val]
+                 | progress
+                    cbn[subst_Frame subst_Tm subst_Val ren_Tm ren_Val]
                  | progress fsimpl ]).
 
 Ltac asimpl := check_no_evars;
                 repeat
                  unfold VarInstance_Val, Var, ids, Ren_Val, Ren1, ren1,
                   Ren_Tm, Ren1, ren1, Up_Val_Val, Up_Val, up_Val, Subst_Val,
-                  Subst1, subst1, Subst_Tm, Subst1, subst1 in *;
+                  Subst1, subst1, Subst_Tm, Subst1, subst1, Subst_Frame,
+                  Subst1, subst1 in *;
                 asimpl'; minimize.
 
 Tactic Notation "asimpl" "in" hyp(J) := revert J; asimpl; intros J.
@@ -1449,21 +1455,17 @@ Module Extra.
 Import
 Core.
 
-Arguments bind {n_Val}.
-
-Arguments box {n_Val}.
+Arguments f_let {n_Val}.
 
 Arguments unfold {n_Val}.
 
-Arguments app {n_Val}.
-
 Arguments case {n_Val}.
-
-Arguments split {n_Val}.
 
 Arguments prj {n_Val}.
 
 Arguments ifz {n_Val}.
+
+Arguments app {n_Val}.
 
 Arguments let_ {n_Val}.
 
@@ -1475,8 +1477,6 @@ Arguments fold {n_Val}.
 
 Arguments rec {n_Val}.
 
-Arguments abs {n_Val}.
-
 Arguments inj {n_Val}.
 
 Arguments prod {n_Val}.
@@ -1484,6 +1484,12 @@ Arguments prod {n_Val}.
 Arguments succ {n_Val}.
 
 Arguments zero {n_Val}.
+
+Arguments abs {n_Val}.
+
+Arguments unit {n_Val}.
+
+#[global] Hint Opaque subst_Frame: rewrite.
 
 #[global] Hint Opaque subst_Tm: rewrite.
 
