rocq/rec/prim.v
@@ -1,0 +1,40 @@
+(** * Imports *)
+
+Require Export rec.reduction.
+
+Open Scope rec_scope.
+Import SyntaxNotations.
+
+(** * Primitive reductions (i.e. beta steps) *)
+
+Reserved Notation "e ~>> e'" (at level 70) .
+
+Inductive primitive : Tm 0 -> Tm 0 -> Prop := 
+  | s_beta : forall (e : Tm 1) (v : Val 0), 
+      app (abs e) v ~>> e[v..]
+  | s_ifz_zero : forall (e1 : Tm 0) (e2 : Tm 1), 
+      ifz zero e1 e2 ~>> e1
+  | s_ifz_succ : forall (e1 : Tm 0) (e2 : Tm 1) (k : Val 0), 
+      ifz (succ k) e1 e2 ~>> e2[k..]
+  | s_prj1 : forall v1 v2 : Val 0, 
+      prj1 (prod v1 v2) ~>> ret v1
+  | s_prj2 : forall v1 v2 : Val 0, 
+      prj2 (prod v1 v2) ~>> ret v2
+  | s_case_inj1 : forall (v : Val 0) (e1 e2 : Tm 1), 
+      case (inj1 v) e1 e2 ~>> e1[v..]
+  | s_case_inj2 : forall (v : Val 0) (e1 e2 : Tm 1), 
+      case (inj2 v) e1 e2 ~>> e2[v..]
+  | s_app_rec : forall (v : Val 1) (v1 : Val 0), 
+      app (rec v) v1 ~>> app v[(rec v)..] v1
+  | s_prj_rec : forall (b : bool) (v : Val 1), 
+      prj b (rec v) ~>> prj b v[(rec v)..]
+  | s_unfold : forall v : Val 0, 
+      unfold (fold v) ~>> ret v 
+where "e ~>> e'" := (primitive e e').
+
+Lemma primitive_deterministic :
+  forall e e1 e2, e ~>> e1 -> e ~>> e2 -> e1 = e2.
+Proof.
+  intros e e1 e2 h1 h2.
+  inversion h1; subst; inversion h2; subst; eauto.
+Qed.
