rocq/rec/stack.v
@@ -1,0 +1,314 @@
+Require Export rec.prim.
+
+Import SyntaxNotations.
+Export Lists.List.ListNotations.
+Open Scope list_scope.
+Open Scope rec_scope.
+
+(** * Refactoring of Small step semantics using primitive reductions *)
+
+Module Small.
+
+Reserved Notation "e1 ~> e2" (at level 70).
+
+Inductive step : Tm 0 -> Tm 0 -> Prop := 
+  | s_prim e1 e2 : 
+    e1 ~>> e2 -> e1 ~> e2
+
+  | s_letv v e : 
+    let_ (ret v) e ~> e [v..]
+
+  | s_let_cong e1 e1' e2 : 
+    e1 ~> e1' ->
+    let_ e1 e2 ~> let_ e1' e2
+where "e1 ~> e2" := (step e1 e2).
+
+Lemma ret_irreducible v : 
+  forall e, not (ret v ~> e).
+Proof.
+  intros e h. inversion h. inversion H. Qed.
+
+Lemma deterministic :
+  forall e e1 e2, e ~> e1 -> e ~> e2 -> e1 = e2.
+Proof. 
+  intros e e1 e2 h1. move: e2.
+  induction h1; intros ? h2; inversion h2; subst; eauto.
+  eapply primitive_deterministic; eauto.
+  all: try match goal with [H : let_ _ _ ~>> _ |- _ ] => inversion H end.
+  assert False. eapply ret_irreducible; eauto. done.
+  assert False. eapply ret_irreducible; eauto. done.
+  erewrite IHh1; eauto.
+Qed.
+
+(** This refactored version is equivalent to our prior version *)
+Lemma equivalent : 
+  forall e e' , e ~> e' <-> rec.reduction.Small.step e e'.
+Proof.
+  intros e e'.
+  split.
+  - intro h; induction h; eauto with rec.
+    inversion H; eauto with rec.
+  - intro h; induction h; eauto using primitive, step.
+Qed. 
+
+(** We have a congruence rule for multistep reduction in the RHS of a let *)
+Lemma let_cong : 
+  forall e1 e1' e2, multi Small.step e1 e1' -> multi Small.step (let_ e1 e2) (let_ e1' e2).
+Proof.
+  intros e1 e1' e2 h. 
+  induction h; eauto using Small.step, multi.
+Qed.
+
+End Small.
+
+
+(** * Refactoring of Big Step semantics *)
+
+Module Big. 
+
+Reserved Notation "e ⇓ v" (at level 70).
+
+Inductive step : Tm 0 -> Val 0 -> Prop := 
+  | s_val v : 
+    ret v ⇓ v
+  | s_prim e1 e2 v : 
+    e1 ~>> e2 ->
+    e2 ⇓ v ->
+    e1 ⇓ v 
+  | s_let v1 e1 e2 v : 
+    e1 ⇓ v1 ->
+    e2 [v1..] ⇓ v ->
+    let_ e1 e2 ⇓ v
+where "e ⇓ v" := (step e v).
+
+(** The big-step semantics is deterministic *)
+Lemma deterministic :
+  forall e v1 v2, e ⇓ v1 -> e ⇓ v2 -> v1 = v2.
+Proof.
+  intros e v1 v2 h1. move: v2.
+  induction h1; intros ? h2; inversion h2; subst.
+  all: eauto.
+  all: try match goal with [ H : ret _ ~>> _ |- _ ] => inversion H end.
+  all: try match goal with [ H : let_ _ _ ~>> _ |- _ ] => inversion H end.
+  eapply primitive_deterministic in H; eauto. subst.  eauto.
+  have EQ: v1 = v0. eapply IHh1_1; eauto. subst.
+  eauto.
+Qed.
+
+End Big.
+
+(** * Big step is equivalent to small step *)
+
+Lemma step_expansion (e1 e2 : Tm 0) (v : Val 0): 
+  Small.step e1 e2 -> Big.step e2 v ->
+  Big.step e1 v.
+Proof.
+(* FILL IN HERE *) Admitted.
+
+Lemma SmallBig : 
+  forall e v, multi Small.step e (ret v) -> Big.step e v.
+Proof. intros e v h. 
+       dependent induction h. 
+(* FILL IN HERE *) Admitted.
+
+Lemma BigSmall : 
+  forall e v, Big.step e v -> multi Small.step e (ret v).
+Proof. 
+  intros e v h.
+  induction h.
+(* FILL IN HERE *) Admitted.
+
+Lemma SmallBig_equivalence : 
+  forall e v, Big.step e v <-> multi Small.step e (ret v).
+Proof. split. eapply BigSmall; eauto. eapply SmallBig; eauto. Qed.
+
+
+(** * Semantics based on an abstract machine with an explicit stack *)
+
+(** A frame corresponds to the [let_cong] rule of the small step semantics.
+   It remembers that after evaluating [e1] we need to continue with evaluting
+   the body of a let expression. This body has a single bound variable. *)
+
+Definition frame   := Frame 0.
+Definition stack   := list frame.
+Definition machine := (stack * Tm 0)%type.
+
+(** An abstract machine is done evaluating when the stack is empty and 
+    the expression is a value. *)
+Inductive final : machine -> Prop := 
+  | final_machine v :
+    final ( [] , ret v ).
+
+Module StackSmall.
+
+Inductive step : machine -> machine -> Prop := 
+  | s_prim k e e' : 
+    e ~>> e' ->
+    step (k , e) (k, e')
+
+  | s_pop k e2 v : 
+    step (f_let e2 :: k, ret v) (k, e2[v..])
+
+  | s_push  k e1 e2 : 
+    step (k , let_ e1 e2 ) (f_let e2 :: k, e1).
+  
+Definition irreducible (m : machine) : Prop := 
+  forall m', not (step m m').
+
+Lemma deterministic :
+  forall m m1 m2, step m m1 -> step m m2 -> m1 = m2.
+Proof.
+  intros m m1 m2 h1 h2. 
+  inversion h1; subst; inversion h2; subst; auto.
+  all: try match goal with [ H : ret _ ~>> _ |- _ ] => inversion H end.
+  all: try match goal with [ H : let_ _ _ ~>> _ |- _ ] => inversion H end.
+  eapply primitive_deterministic in H; eauto. subst. auto.
+Qed.
+
+End StackSmall.
+
+Module StackBig.
+  
+(* Big-step machine semantics *)
+Inductive step : machine -> Val 0 -> Prop := 
+  | s_final v : 
+    step ([], ret v) v
+
+  | s_prim k e e' v : 
+    e ~>> e' ->
+    step (k, e') v ->
+    step (k , e) v
+
+  | s_pop k e2 v1 v : 
+    step (k, e2[v1..]) v  ->
+    step (f_let e2 :: k, ret v1) v
+
+  | s_push  k e1 e2 v : 
+    step (f_let e2 :: k, e1) v ->
+    step (k , let_ e1 e2 ) v .
+
+End StackBig.
+
+
+
+Module Notations.
+Infix "~>" := Small.step (at level 70) : rec_scope.
+Infix "~>*" := (multi Small.step) (at level 70) : rec_scope.
+Infix "⇓"  := Big.step (at level 70) : rec_scope. 
+Infix "↦"  := StackSmall.step (at level 70) : rec_scope.
+Infix "↦*"  := (multi StackSmall.step) (at level 70) : rec_scope.
+Infix "⇊"  := StackBig.step (at level 70) : rec_scope.   (* \downdownarrows *) 
+End Notations.
+
+Import Notations.
+
+(** * Machine semantics is the same as the original semantics *)
+
+Lemma bigstep_completeness e v :
+  e ⇓ v -> 
+  forall s : stack, (s, e) ↦* (s, ret v).
+Proof.
+  intro h.
+  induction h. 
+(* FILL IN HERE *) Admitted.
+
+(* PFPL 28.2 *)
+Corollary smallstep_completeness e v: 
+  e ~>* (ret v) -> ([], e) ↦* ([], ret v).
+Proof.
+  intros h.
+  generalize ([] : stack).
+  apply SmallBig in h.
+  eapply bigstep_completeness; auto.
+Qed.
+
+Fixpoint unravel (s : stack) (e : Tm 0) : Tm 0 := 
+ match s with 
+  | [] => e 
+  | f_let e2 :: k => unravel k (let_ e e2)
+  end.
+
+(** The stack indicates the next reduction step that should happen *)
+Lemma stack_cong k e e': 
+  (e ~> e') -> unravel k e ~> unravel k e'.
+Proof. 
+  move: e e'.
+  induction k.
+  - intros. cbn. done.
+  - intros. 
+    destruct a. cbn.
+    eapply IHk.
+    eapply Small.s_let_cong. auto.
+Qed.
+
+Lemma unravel_step {k e k' e'} :
+  (k, e) ↦ (k', e') -> (unravel k e) ~>* (unravel k' e').
+Proof.
+  intro h.
+  dependent induction h; subst.
+  - eapply ms_one. eapply stack_cong. eapply Small.s_prim; auto.
+  - cbn. eapply ms_one. eapply stack_cong.  eapply Small.s_letv; eauto.
+  - cbn. eapply ms_refl.
+Qed.
+
+Lemma unravel_multistep s s' e v: 
+  (s, e) ↦* (s', ret v) -> unravel s e ~>* unravel s' (ret v).
+Proof.
+  intro h. dependent induction h.
+  - eapply ms_refl.
+  - destruct e2 as [s2 e2].
+    specialize (IHh s2 s' e2 v ltac:(eauto) ltac:(eauto)).
+    eapply ms_app. eapply unravel_step; eauto.
+    eauto.
+Qed.
+    
+Lemma smallstep_soundness e v: 
+  ([], e) ↦* ([], ret v) -> e ~>* (ret v).
+Proof.
+  eapply unravel_multistep; eauto.
+Qed.
+
+Lemma small_machine_correctness e v:
+  ([], e) ↦* ([], ret v) <-> e ~>* ret v.
+Proof.
+  split. eapply smallstep_soundness. eapply smallstep_completeness.
+Qed.
+
+(** * Big machine correctness *)
+
+Lemma small_big_completeness s e v: 
+  (s, e) ↦* ([], ret v) -> (s, e) ⇊ v.
+Proof.
+  intro h.
+  dependent induction h.
+  - eapply StackBig.s_final.
+  - inversion H; subst.
+    + eapply StackBig.s_prim; eauto. 
+    + eapply StackBig.s_pop; eauto.
+    + eapply StackBig.s_push; eauto.
+Qed.    
+
+Lemma small_big_soundness s e v : 
+  (s, e) ⇊ v -> (s, e) ↦* ([], ret v).
+Proof.
+  intro h.
+  dependent induction h.
+  - eapply ms_refl.
+  - eapply ms_trans. eapply StackSmall.s_prim; eauto. eauto.
+  - eapply ms_trans. eapply StackSmall.s_pop. eauto.
+  - eapply ms_trans. eapply StackSmall.s_push. eauto.
+Qed.
+
+Lemma small_big_correctness e v:
+  ([], e) ↦* ([], ret v) <-> ([], e) ⇊ v.
+Proof.
+  split. eapply small_big_completeness. eapply small_big_soundness.
+Qed.
+
+Lemma big_correctness e v :
+  e ⇓ v <-> ([], e) ⇊ v.
+Proof.
+  rewrite SmallBig_equivalence. 
+  rewrite <- small_big_correctness.
+  rewrite small_machine_correctness. done.
+Qed.
